pulse/lib/steel/pulse/Pulse.Checker.Framing.fst
@@ -12,6 +12,7 @@ module P = Pulse.Syntax.Printer
 module RTB = FStar.Tactics.Builtins
 module FV = Pulse.Typing.FV
 module Metatheory = Pulse.Typing.Metatheory
+module VP = Pulse.Checker.VPropEquiv
 
 let print_vprop_l (vps:list term) : T.Tac string =
   Printf.sprintf "[%s]"
@@ -22,99 +23,6 @@ let print_framing_failure ff =
     (print_vprop_l ff.unmatched_preconditions)
     (print_vprop_l ff.remaining_context)
 
-let rec vprop_as_list (vp:term)
-  : list term
-  = match vp with
-    | Tm_Emp -> []
-    | Tm_Star vp0 vp1 -> vprop_as_list vp0 @ vprop_as_list vp1
-    | _ -> [vp]
-
-let rec list_as_vprop (vps:list term)
-  : term
-  = match vps with
-    | [] -> Tm_Emp
-    | hd::tl -> Tm_Star hd (list_as_vprop tl)
-
-let canon_vprop (vp:term)
-  : term
-  = list_as_vprop (vprop_as_list vp)
-
-let rec list_as_vprop_append g (vp0 vp1:list term)
-  : GTot (vprop_equiv g (list_as_vprop (vp0 @ vp1))
-                        (Tm_Star (list_as_vprop vp0) 
-                                 (list_as_vprop vp1)))
-         (decreases vp0)
-  = match vp0 with
-    | [] -> 
-      let v : vprop_equiv g (list_as_vprop vp1)
-                            (Tm_Star Tm_Emp (list_as_vprop vp1)) = VE_Sym _ _ _ (VE_Unit _ _)
-      in
-      v
-    | hd::tl ->
-      let tl_vp1 = list_as_vprop_append g tl vp1 in
-      let d : vprop_equiv g (list_as_vprop (vp0 @ vp1))
-                              (Tm_Star hd (Tm_Star (list_as_vprop tl) (list_as_vprop vp1)))
-            = VE_Ctxt _ _ _ _ _ (VE_Refl _ hd) tl_vp1
-      in
-      let d : vprop_equiv g (list_as_vprop (vp0 @ vp1))
-                              (Tm_Star (Tm_Star hd (list_as_vprop tl)) (list_as_vprop vp1))
-            = VE_Trans _ _ _ _ d (VE_Assoc _ _ _ _) in
-      d
-
-let list_as_vprop_comm g (vp0 vp1:list term)
-  : GTot (vprop_equiv g (list_as_vprop (vp0 @ vp1))
-                        (list_as_vprop (vp1 @ vp0)))
-  = let d1 : _ = list_as_vprop_append g vp0 vp1 in
-    let d2 : _ = VE_Sym _ _ _ (list_as_vprop_append g vp1 vp0) in
-    let d1 : _ = VE_Trans _ _ _ _ d1 (VE_Comm _ _ _) in
-    VE_Trans _ _ _ _ d1 d2
-
-let list_as_vprop_assoc g (vp0 vp1 vp2:list term)
-  : GTot (vprop_equiv g (list_as_vprop (vp0 @ (vp1 @ vp2)))
-                        (list_as_vprop ((vp0 @ vp1) @ vp2)))
-  = List.Tot.append_assoc vp0 vp1 vp2;
-    VE_Refl _ _
-    
-let list_as_vprop_ctx g (vp0 vp1 vp2:list term)
-  (d:vprop_equiv g (list_as_vprop vp0) (list_as_vprop vp1))
-  : GTot (vprop_equiv g (list_as_vprop (vp0 @ vp2)) (list_as_vprop (vp1 @ vp2)))
-
-  = let split_app = list_as_vprop_append _ vp0 vp2 in
-    let ctxt = VE_Ctxt _ _ _ _ _ d (VE_Refl _ (list_as_vprop vp2)) in
-    let split_app2 = VE_Sym _ _ _ (list_as_vprop_append _ vp1 vp2) in
-    VE_Trans _ _ _ _ split_app (VE_Trans _ _ _ _ ctxt split_app2)
-  
-
-let list_as_vprop_singleton g
-  (p q:term)
-  (d:vprop_equiv g p q)
-  : GTot (vprop_equiv g (list_as_vprop [p]) (list_as_vprop [q]))
-  = VE_Ctxt _ p Tm_Emp q Tm_Emp d (VE_Refl _ Tm_Emp)
-
-let rec vprop_list_equiv (g:env)
-                         (vp:term)
-  : GTot (vprop_equiv g vp (canon_vprop vp))
-         (decreases vp)
-  = match vp with
-    | Tm_Emp -> VE_Refl _ _
-    | Tm_Star vp0 vp1 ->
-      let eq0 = vprop_list_equiv g vp0 in
-      let eq1 = vprop_list_equiv g vp1 in      
-      let app_eq
-        : vprop_equiv _ (canon_vprop vp) (Tm_Star (canon_vprop vp0) (canon_vprop vp1))
-        = list_as_vprop_append g (vprop_as_list vp0) (vprop_as_list vp1)
-      in
-      let step
-        : vprop_equiv _ vp (Tm_Star (canon_vprop vp0) (canon_vprop vp1))
-        = VE_Ctxt _ _ _ _ _ eq0 eq1
-      in
-      VE_Trans _ _ _ _ step (VE_Sym _ _ _ app_eq)
-      
-    | _ -> 
-      VE_Sym _ _ _
-        (VE_Trans _ _ _ _ (VE_Comm g vp Tm_Emp) (VE_Unit _ vp))
-
-module L = FStar.List.Tot.Base
 
 let equational (t:term) : bool =
   match t with
@@ -164,34 +72,11 @@ let rec maybe_split_one_vprop g (p:term) (qs:list term)
            | None -> None
            | Some (| l, q', d, r |) -> Some (| q::l, q', d, r |)
 
-let vprop_equiv_swap_equiv (g:_) (l0 l2:list term)
-  (p q:term) (d_p_q:vprop_equiv g p q)
-  : GTot (vprop_equiv g (list_as_vprop ((l0 @ [q]) @ l2))
-                          (list_as_vprop ([p] @ (l0 @ l2)))) =
-  let d : vprop_equiv g (list_as_vprop ((l0 @ [q]) @ l2))
-                          (list_as_vprop (([q] @ l0) @ l2))
-    = list_as_vprop_ctx g (l0 @ [q]) ([q] @ l0) l2 (list_as_vprop_comm g l0 [q]) in
-  let d' : vprop_equiv g (list_as_vprop (([q] @ l0) @ l2))
-                           (list_as_vprop ([q] @ (l0 @ l2)))
-    = List.Tot.append_assoc [q] l0 l2;
-      VE_Refl _ _ in
-  let d : vprop_equiv g (list_as_vprop ((l0 @ [q]) @ l2))
-                          (list_as_vprop ([q] @ (l0 @ l2)))
-    = VE_Trans _ _ _ _ d d' in
-  let d_q_p = VE_Sym _ _ _ d_p_q in
-  let d' : vprop_equiv g (list_as_vprop [q]) (list_as_vprop [p]) =
-    list_as_vprop_singleton _ _ _ d_q_p in
-  let d' : vprop_equiv g (list_as_vprop ([q] @ (l0 @ l2)))
-                           (list_as_vprop ([p] @ (l0 @ l2)))
-    = list_as_vprop_ctx g [q] [p] (l0 @ l2) d' in
-  VE_Trans _ _ _ _ d d'
-
 let framing_success g req ctxt =
   (frame:list term &
-   vprop_equiv g (list_as_vprop (req @ frame)) (list_as_vprop ctxt))
+   vprop_equiv g (VP.list_as_vprop (req @ frame)) (VP.list_as_vprop ctxt))
    
 let try_frame_result g req ctxt = either (framing_success g req ctxt) framing_failure
-
 
 let mk_framing_failure #g #req #req' #ctxt #ctxt'
                        (unmatched_pre:term)
@@ -210,7 +95,7 @@ let mk_framing_failure #g #req #req' #ctxt #ctxt'
 let rec try_split_vprop g (req:list term) (ctxt:list term)
   : T.Tac 
     (either (frame:list term &
-             vprop_equiv g (list_as_vprop (req @ frame)) (list_as_vprop ctxt))
+             vprop_equiv g (VP.list_as_vprop (req @ frame)) (VP.list_as_vprop ctxt))
             framing_failure)
   = match req with
     | [] -> Inl (| ctxt, VE_Refl g _ |)
@@ -221,22 +106,22 @@ let rec try_split_vprop g (req:list term) (ctxt:list term)
 
       | Some (| l, q, d, r |) -> 
         let d1
-          : vprop_equiv g (list_as_vprop ctxt)
-                            (list_as_vprop (hd :: (l@r)))
-          = vprop_equiv_swap_equiv g l r hd q d
+          : vprop_equiv g (VP.list_as_vprop ctxt)
+                          (VP.list_as_vprop (hd :: (l@r)))
+          = VP.vprop_equiv_swap_equiv g l r hd q d
         in
         match try_split_vprop g tl (l @ r) with
         | Inr failure -> Inr failure
         | Inl (| frame, d |) ->
           let d
-            : vprop_equiv g (list_as_vprop (tl @ frame))
-                              (list_as_vprop (l @ r))
+            : vprop_equiv g (VP.list_as_vprop (tl @ frame))
+                            (VP.list_as_vprop (l @ r))
             = d
           in
           let dd
-            : vprop_equiv g (list_as_vprop (req @ frame))
-                              (list_as_vprop (hd :: (l @ r)))
-            = VE_Ctxt _ _ _ _ _ (VE_Refl _ hd) d
+            : vprop_equiv g (VP.list_as_vprop ((hd::tl) @ frame))
+                            (VP.list_as_vprop (hd :: (l @ r)))
+            = VP.list_as_vprop_ctx g [hd] [hd] _ _ (VE_Refl _ _) d
           in
           let ddd = VE_Trans _ _ _ _ dd (VE_Sym _ _ _ d1) in
           Inl (| frame, ddd |)
@@ -250,36 +135,19 @@ let split_vprop (g:env)
                     tot_typing g frame Tm_VProp &
                     vprop_equiv g (Tm_Star req frame) ctxt)
                    framing_failure)
-   = let ctxt_l = vprop_as_list ctxt in
-     let req_l = vprop_as_list req in
+   = let ctxt_l = VP.vprop_as_list ctxt in
+     let req_l = VP.vprop_as_list req in
      match try_split_vprop g req_l ctxt_l with
      | Inr failure -> 
        Inr failure 
      | Inl (| frame, veq |) ->
-       let d1 
-         : vprop_equiv _ (Tm_Star (canon_vprop req) (list_as_vprop frame))
-                           (list_as_vprop (req_l @ frame))
-         = VE_Sym _ _ _ (list_as_vprop_append g req_l frame)
-       in
-       let d1 
-         : vprop_equiv _ (Tm_Star req (list_as_vprop frame))
-                           (list_as_vprop (req_l @ frame))
-         = VE_Trans _ _ _ _ (VE_Ctxt _ _ _ _ _ (vprop_list_equiv g req) (VE_Refl _ _)) d1
-       in
-       let d : vprop_equiv  _ (Tm_Star req (list_as_vprop frame))
-                             (canon_vprop ctxt) =
-           VE_Trans _ _ _ _ d1 veq
-       in
-       let d : vprop_equiv _ (Tm_Star req (list_as_vprop frame))
-                               ctxt =
-         VE_Trans _ _ _ _ d (VE_Sym _ _ _ (vprop_list_equiv g ctxt))
-       in
-       let typing : tot_typing g (list_as_vprop frame) Tm_VProp = 
-         let fwd, bk = vprop_equiv_typing d in
+       let d = VP.vprop_equiv_split_frame g ctxt req frame veq in
+       let typing : tot_typing g (VP.list_as_vprop frame) Tm_VProp = 
+         let fwd, bk = VP.vprop_equiv_typing d in
          let star_typing = bk ctxt_typing in
          snd (star_typing_inversion star_typing)
        in
-       Inl (| list_as_vprop frame, typing, d |)
+       Inl (| VP.list_as_vprop frame, typing, d |)
 
 let rec check_equiv_emp (g:env) (vp:term)
   : option (vprop_equiv g vp Tm_Emp)
@@ -338,11 +206,6 @@ let freevars_comp_post (c:comp { stateful_comp c })
   = ()
 
 #push-options "--z3rlimit_factor 20 --query_stats --fuel 4 --ifuel 2 --query_stats"
-
-let frame_for_req_in_ctxt (g:env) (ctxt:term) (req:term)
-   = (frame:term &
-      tot_typing g frame Tm_VProp &
-      vprop_equiv g (Tm_Star req frame) ctxt)
 
   
 let check_frameable (#g:env)
