pulse/lib/steel/pulse/Pulse.Checker.Auto.ElimExists.fsti
@@ -1,0 +1,11 @@
+module Pulse.Checker.Auto.ElimExists
+open Pulse.Syntax
+open Pulse.Checker.Common
+open Pulse.Typing
+module T = FStar.Tactics
+
+val elim_exists (#g:env) (#ctxt:term) (ctxt_typing:tot_typing g ctxt Tm_VProp)
+   : T.Tac (g':env { env_extends g' g } &
+            ctxt':term &
+            tot_typing g' ctxt' Tm_VProp &
+            continuation_elaborator g ctxt g' ctxt')
