pulse/lib/steel/pulse/Pulse.Checker.Auto.ElimPure.fst
@@ -1,0 +1,157 @@
+module Pulse.Checker.Auto.ElimPure
+module RT = FStar.Reflection.Typing
+module R = FStar.Reflection
+module L = FStar.List.Tot
+module T = FStar.Tactics
+open FStar.List.Tot
+open Pulse.Syntax
+open Pulse.Checker.Pure
+open Pulse.Checker.Common
+open Pulse.Typing
+module Metatheory = Pulse.Typing.Metatheory
+module VP = Pulse.Checker.VPropEquiv
+
+let k_elab_trans (#g0 #g1 #g2:env) (#ctxt0 #ctxt1 #ctxt2:term)
+                 (k0:continuation_elaborator g0 ctxt0 g1 ctxt1)
+                 (k1:continuation_elaborator g1 ctxt1 g2 ctxt2)
+   : continuation_elaborator g0 ctxt0 g2 ctxt2
+   = fun post_hint res -> k0 post_hint (k1 post_hint res)
+
+let elim_one_pure (#g:env) (ctxt:term) (p:term)
+                  (ctxt_typing:tot_typing g (Tm_Star ctxt (Tm_Pure p)) Tm_VProp)
+   : T.Tac (g':env { env_extends g' g } &
+            tot_typing g' ctxt Tm_VProp &
+            continuation_elaborator g (Tm_Star ctxt (Tm_Pure p)) g' ctxt)
+   = admit()
+                  
+let rec elim_pure_right (#g:env) (#ctxt:term) (ctxt_typing:tot_typing g ctxt Tm_VProp)
+   : T.Tac (g':env { env_extends g' g } &
+            ctxt':term &
+            tot_typing g' ctxt' Tm_VProp &
+            continuation_elaborator g ctxt g' ctxt')
+   = match ctxt with
+     | Tm_Star ctxt' (Tm_Pure p) ->
+       let (| g', ctxt_typing', k |) = elim_one_pure ctxt' p ctxt_typing in
+       let (| g'', ctxt'', ctxt_typing'', k' |) = elim_pure_right ctxt_typing' in
+       (| g'', ctxt'', ctxt_typing'', k_elab_trans k k' |)
+     | _ ->
+        extends_env_refl g;
+        let k : continuation_elaborator g ctxt g ctxt = fun post_hint res -> res in
+       (| g, ctxt, ctxt_typing, k |)
+
+module F = Pulse.Checker.Framing
+open Pulse.Checker.VPropEquiv
+                        
+let rec canon_pure_right_aux (g:env) (vps:list vprop)
+  : vps':list vprop &
+    pures:list vprop &
+    vprop_equiv g (list_as_vprop vps) (list_as_vprop (vps' @ pures))
+  = match vps with
+    | [] -> (| [], [], VE_Refl _ _ |)
+    | [Tm_Pure p] -> (| [], [Tm_Pure p], VE_Refl _ _ |)
+    | Tm_Pure p :: rest -> 
+      let (| vps', pures, v_eq |) = canon_pure_right_aux g rest in
+      let v_eq
+         : vprop_equiv g (list_as_vprop vps)
+                         (list_as_vprop ((Tm_Pure p) :: (vps' @ pures)))
+         = list_as_vprop_ctx g [Tm_Pure p] _ rest (vps' @ pures) (VE_Refl _ _) v_eq    
+      in  
+      let v_eq
+         : vprop_equiv g (list_as_vprop vps)
+                         (list_as_vprop ((vps'@[Tm_Pure p]) @ pures))
+         = VE_Trans _ _ _ _ v_eq (VE_Sym _ _ _ (vprop_equiv_swap_equiv _ _ _ (Tm_Pure p) _ (VE_Refl _ _)))
+      in
+      let v_eq 
+        :  vprop_equiv g (list_as_vprop vps)
+                         (list_as_vprop (vps'@(Tm_Pure p::pures)))
+        = VE_Trans _ _ _ _ v_eq (VE_Sym _ _ _ (list_as_vprop_assoc _ _ _ _)) in
+      (| vps', Tm_Pure p :: pures, v_eq |)
+    | hd::rest ->
+      let (| vps', pures, v_eq |) = canon_pure_right_aux g rest in
+      let v_eq = list_as_vprop_ctx g [hd] _ _ _ (VE_Refl _ _) v_eq in
+      (| hd::vps', pures, v_eq |)
+
+let vprop_equiv_typing_fwd (#g:env) (#ctxt:_) (ctxt_typing:tot_typing g ctxt Tm_VProp)
+                           (#p:_) (d:vprop_equiv g ctxt p)
+  : tot_typing g p Tm_VProp 
+  = let fwd, _ = vprop_equiv_typing d in
+    fwd ctxt_typing
+
+let canon_pure_right (#g:env) (#ctxt:term) (ctxt_typing:tot_typing g ctxt Tm_VProp)
+  : (ctxt':term &
+     tot_typing g ctxt' Tm_VProp &
+     continuation_elaborator g ctxt g ctxt')
+  = let ctxt' = canon_vprop ctxt in
+    let (| vps', pures, veq |) = canon_pure_right_aux g (vprop_as_list ctxt) in
+    let veq : vprop_equiv g ctxt (list_as_vprop (vps'@pures)) =
+        VE_Trans _ _ _ _ (vprop_list_equiv g ctxt) veq
+    in
+    let veq' :vprop_equiv g (Tm_Star (list_as_vprop (vps'@pures)) Tm_Emp) ctxt =
+        VE_Trans _ _ _ _ (VE_Comm _ _ _) (VE_Trans _ _ _ _ (VE_Unit _ _) (VE_Sym _ _ _ veq))
+    in 
+    let framing_token : Pulse.Checker.Framing.frame_for_req_in_ctxt g ctxt (list_as_vprop (vps'@pures)) = 
+        (| Tm_Emp, emp_typing, veq' |) in
+    let k : continuation_elaborator g ctxt g (list_as_vprop (vps'@pures)) =
+        fun post_hint res -> 
+            let (| st, c, st_d |) = res in
+            if not (stateful_comp c)
+            then T.fail "Unexpected non-stateful comp in continuation elaborate"
+            else (
+                let (| c', st_d' |) = Pulse.Checker.Framing.apply_frame ctxt_typing st_d framing_token in
+                (| _, _, st_d' |)
+            )
+    in
+    (| _, vprop_equiv_typing_fwd ctxt_typing veq, k |)
+
+  
+                
+let elim_pure (#g:env) (#ctxt:term) (ctxt_typing:tot_typing g ctxt Tm_VProp)
+   : T.Tac (g':env { env_extends g' g } &
+            ctxt':term &
+            tot_typing g' ctxt' Tm_VProp &
+            continuation_elaborator g ctxt g' ctxt')
+   = let (| ctxt', ctxt'_typing, k |) = canon_pure_right ctxt_typing in
+     let (| g', ctxt'', ctxt''_typing, k' |) = elim_pure_right ctxt'_typing in
+     (| g', ctxt'', ctxt''_typing, k_elab_trans k k' |)
+     
+
+
+
+
+// let rec maybe_add_elims
+//            (g:env)
+//            (ctxt:list term)
+//            (t:st_term)
+//   : T.Tac st_term
+//   = let wr t' = { term = t'; range = t.range } in
+//     match ctxt with
+//     | [] -> t
+//     | Tm_ExistsSL u ty b se :: rest ->
+//       let e = wr (Tm_Protect { t = wr (Tm_ElimExists { p = Tm_ExistsSL u ty b se }) }) in
+//       let x = fresh g in
+//       let px = v_as_nv x in
+//       let g = extend x (Inl ty) g in
+//       let b = open_term_nv b px in
+//       let t = maybe_add_elims g [b] t in
+//       let t = close_st_term t x in
+//       let t = Tm_Bind { binder = default_binder_annot;
+//                         head = e;
+//                         body = wr (Tm_Protect { t }) } in
+//       maybe_add_elims g rest (wr t)
+//     | Tm_Pure p :: rest ->
+//       let elim_pure_tm = 
+//         wr (Tm_STApp { head = tm_fvar (as_fv elim_pure_explicit_lid);
+//                        arg_qual = None;
+//                        arg = p })
+//       in
+//       wr (
+//         Tm_Bind { binder = default_binder_annot;
+//                   head = wr (Tm_Protect { t = elim_pure_tm } );
+//                   body = wr (Tm_Protect { t = maybe_add_elims g rest t }) }
+//       )
+
+//     | Tm_Star p q :: rest ->
+//       maybe_add_elims g (p :: q :: rest) t    
+      
+//     | _ :: rest ->
+//       maybe_add_elims g rest t
