pulse/lib/steel/pulse/Pulse.Checker.Auto.ElimPure.fsti
@@ -1,0 +1,17 @@
+module Pulse.Checker.Auto.ElimPure
+module RT = FStar.Reflection.Typing
+module R = FStar.Reflection
+module L = FStar.List.Tot
+module T = FStar.Tactics
+open FStar.List.Tot
+open Pulse.Syntax
+open Pulse.Checker.Pure
+open Pulse.Checker.Common
+open Pulse.Typing
+module Metatheory = Pulse.Typing.Metatheory
+
+val elim_pure (#g:env) (#ctxt:term) (ctxt_typing:tot_typing g ctxt Tm_VProp)
+   : T.Tac (g':env { env_extends g' g } &
+            ctxt':term &
+            tot_typing g' ctxt' Tm_VProp &
+            continuation_elaborator g ctxt g' ctxt')
